tests/CountBy/ListProofs.v
@@ -49,7 +49,7 @@ Definition addNSpec {n} (a b : list (Bvector n)) : list (Bvector n) :=
 
 Local Ltac seqsimpl_step :=
   first [ progress cbn beta iota delta
-                   [fst snd hd sequential loopSeq' loop SequentialCombSemantics]
+                   [fst snd hd sequential loopSeq' loop SequentialSemantics]
         | progress cbv beta iota delta [loopSeq]; seqsimpl_step
         | progress autorewrite with seqsimpl
         | progress destruct_pair_let
@@ -64,7 +64,7 @@ Hint Rewrite addNCorrect using solve [eauto] : seqsimpl.
 
 Lemma countForkStep:
   forall (i : Bvector 8) (s : Bvector 8),
-    sequential (countFork (semantics:=SequentialCombSemantics) ([i], [s]))
+    sequential (countFork ([i], [s]))
     = (countBySpec' s [i], countBySpec' s [i]).
 Proof.
   intros; cbv [countFork countBySpec'].
@@ -74,7 +74,7 @@ Hint Rewrite countForkStep using solve [eauto] : seqsimpl.
 
 Lemma countForkCorrect:
   forall (i : list (Bvector 8)) (s : Bvector 8),
-    sequential (loopSeq' (countFork (semantics:=SequentialCombSemantics)) i [s])
+    sequential (loopSeq' (countFork (combsemantics:=SequentialCombSemantics)) i [s])
     = countBySpec' s i.
 Proof.
   cbv [sequential]; induction i; intros; [ reflexivity | ].
@@ -86,5 +86,5 @@ Lemma countByCorrect: forall (i : list (Bvector 8)),
                       sequential (countBy i) = countBySpec i.
 Proof.
   intros; cbv [countBy countBySpec].
-  seqsimpl; reflexivity.
+  seqsimpl. reflexivity.
 Qed.
